
\documentclass[12pt]{article}\usepackage{amsmath}
\usepackage{graphicx}
\usepackage{fancyhdr}
\usepackage{lastpage}
\pagestyle{fancy}
\lhead{\footnotesize \parbox{11cm}{Joel Anna} }
%\lfoot{\footnotesize \parbox{11cm}{\textit{2}}}
\cfoot{}
\rhead{\footnotesize HW3:  \thepage\ of \pageref{LastPage}}
%\rfoot{\footnotesize Page \thepage\ of \pageref{LastPage}}
\renewcommand{\headheight}{24pt}
%\renewcommand{\footrulewidth}{0.4pt}

\begin{document}
\author{Joel Anna<annajoel@pdx.edu>}
\noindent
\underline{Question 1:}\\
$near = -2. \;\; far = -6. \;\; left = -2. \;\; right = 6.$
$top = 4. \;\; bottom = -4$\\
definition:\\
$\begin{bmatrix}
x_{canonical}\\
y_{canonical}\\
z_{canonical}\\
1
\end{bmatrix}$=
$\begin{bmatrix}
\;\; \frac{2}{r-l}&\;\; 0&\;\; 0&\;\; \frac{-(r+l)}{r-l}\\
\;\; 0 &\;\; \frac{2}{t-b}&\;\; 0&\;\; \frac{-(t+b)}{t-b}\\
\;\; 0&\;\; 0 &\;\; \frac{2}{n-f}&\;\; \frac{-(n+f)}{n-f}\\
 \;\;0&\;\; 0&\;\; 0&\;\; 1\\
\end{bmatrix}$
$\begin{bmatrix}
x_{view}\\
y_{view}\\
z_{view}\\
1
\end{bmatrix}$\\
$\begin{bmatrix}
x_{canonical}\\
y_{canonical}\\
z_{canonical}\\
1
\end{bmatrix}$=
$\begin{bmatrix}
\;\; \frac{2}{6-(-2)}&\;\; 0&\;\; 0&\;\; \frac{-(6+(-2)}{6-(-2}\\
\;\; 0 &\;\; \frac{2}{4-(-4)}&\;\; 0&\;\; \frac{-(4+(-4))}{4-(-4)}\\
\;\; 0&\;\; 0 &\;\; \frac{2}{(-2)-(-6)}&\;\; \frac{-((-2)+(-6))}{(-2)-(-6)}\\
 \;\;0&\;\; 0&\;\; 0&\;\; 1\\
\end{bmatrix}$
$\begin{bmatrix}
x_{view}\\
y_{view}\\
z_{view}\\
1
\end{bmatrix}$\\
$\begin{bmatrix}
x_{canonical}\\
y_{canonical}\\
z_{canonical}\\
1
\end{bmatrix}$=
$\begin{bmatrix}
\;\; \frac{1}{4}&\;\; 0&\;\; 0&\;\; \frac{-1}{2}\\
\;\; 0 &\;\; \frac{1}{4}&\;\; 0&\;\; 0\\
\;\; 0&\;\; 0 &\;\; \frac{1}{2}&\;\; \frac{4}{3}\\
 \;\;0&\;\; 0&\;\; 0&\;\; 1\\
\end{bmatrix}$
$\begin{bmatrix}
x_{view}\\
y_{view}\\
z_{view}\\
1
\end{bmatrix}$\\
\underline{Question 2:}\\
a:\\
$P(x_v, y_v, z_v) = (100,20,20); \;\;d = 10$\\
$\frac{x_s}{d}=\frac{x_v}{z_v} = \frac{100}{20} = 5$\\
$x_s = 5\cdot d = 50$\\
$\frac{y_s}{d}=\frac{y_v}{z_v} = \frac{20}{20} = 1$\\
$y_s = 1\cdot d = 10$\\
$P(x_s, y_s) = (50,10)$\\
b:\\
$P(x_s, y_s) = (20,10)$\\
$\frac{x_v}{z_v} = \frac{x_s}{d}= 2\;\;\;$
$x_v = 2\cdot z_v$\\
$\frac{y_v}{z_v} = \frac{y_s}{d}= 1\;\;\;$
$y_v = 1\cdot z_v$\\
There are 3 variables, but only 2 equations, we cannot uniquely determine the 3D point's coordinate because of this.\\
Any point on the line $(2\cdot z_v, 1\cdot z_v, z_v)$ could be the original coordinate.\\
\pagebreak\\
\underline{Question 3:}\\
\textbf{($f$ inside $s$) over $b$\\}
values in r,g,b,a\\
$f$ =
$\begin{bmatrix}
\;\; 1,1,1,1 \;\; & \;\; 1,1,1,1 \;\; & \;\; 1,1,1,1 \;\;\\
\;\; 1,1,1,1 \;\; & \;\; 1,1,1,1 \;\; & \;\; 1,1,1,1 \;\;\\
\;\; 1,1,1,1 \;\; & \;\; 1,1,1,1 \;\; & \;\; 1,1,1,1 \;\;\\
\end{bmatrix}$
$s$ = 
$\begin{bmatrix}
\;\; 1,1,1,1 \;\; & \;\; 0,0,0,0  \;\; & \;\; 1,1,1,1 \;\;\\
\;\; 0,0,0,0 \;\; & \;\; 1,1,1,1  \;\; & \;\; 0,0,0,0  \;\;\\
\;\; 1,1,1,1 \;\; & \;\; 0,0,0,0  \;\; & \;\; 1,1,1,1 \;\;\\
\end{bmatrix}$
b = 
$\begin{bmatrix}
\;\; 1,0,0,1 \;\; & \;\; 1,0,0,1  \;\; & \;\; 1,0,0,1 \;\;\\
\;\; 1,0,0,1 \;\; & \;\; 1,0,0,1  \;\; & \;\; 1,0,0,1 \;\;\\
\;\; 1,0,0,1 \;\; & \;\; 1,0,0,1  \;\; & \;\; 1,0,0,1 \;\;\\
\end{bmatrix}$\\
($f$ inside $s$) = $f_1$ = $\alpha_s c_f$ =
$\begin{bmatrix}
\;\; 1,1,1,1 \;\; & \;\; 0,0,0,0  \;\; & \;\; 1,1,1,1 \;\;\\
\;\; 0,0,0,0 \;\; & \;\; 1,1,1,1  \;\; & \;\; 0,0,0,0  \;\;\\
\;\; 1,1,1,1 \;\; & \;\; 0,0,0,0  \;\; & \;\; 1,1,1,1 \;\;\\
\end{bmatrix}$\\
$f_1$ over $b$ = $\alpha_s c_f$ = $c_{f_1} + (1-\alpha_{f_1})c_b$=\\
$\begin{bmatrix}
\;\; 1,1,1,1 \;\; & \;\; 0,0,0,0  \;\; & \;\; 1,1,1,1 \;\;\\
\;\; 0,0,0,0 \;\; & \;\; 1,1,1,1  \;\; & \;\; 0,0,0,0  \;\;\\
\;\; 1,1,1,1 \;\; & \;\; 0,0,0,0  \;\; & \;\; 1,1,1,1 \;\;\\
\end{bmatrix}$+$\begin{bmatrix}
\;\; 0,0,0,0 \;\; & \;\; 1,0,0,1  \;\; & \;\;  0,0,0,0 \;\;\\
\;\; 1,0,0,1 \;\; & \;\; 0,0,0,0  \;\; & \;\; 1,0,0,1 \;\;\\
\;\; 0,0,0,0 \;\; & \;\; 1,0,0,1  \;\; & \;\;  0,0,0,0 \;\;\\
\end{bmatrix}$=\\\\
$\begin{bmatrix}
\;\; 1,1,1,1 \;\; & \;\; 1,0,0,1  \;\; & \;\; 1,1,1,1 \;\;\\
\;\; 1,0,0,1 \;\; & \;\; 1,1,1,1  \;\; & \;\; 1,0,0,1  \;\;\\
\;\; 1,1,1,1 \;\; & \;\; 1,0,0,1  \;\; & \;\; 1,1,1,1 \;\;\\
\end{bmatrix}$
\pagebreak\\
\underline{Question 4:}\\
$\begin{bmatrix}
u\\
v\\
1
\end{bmatrix}$=
$\begin{bmatrix}
\;\; a \;\; & \;\; b \;\; & \;\; c \;\;\\
\;\; d \;\; & \;\; e \;\; & \;\; f \;\;\\
\;\; 0 \;\; & \;\; 0 \;\; & \;\; 1 \;\;\\
\end{bmatrix}$
$\begin{bmatrix}
x\\
y\\
1
\end{bmatrix}$\\
$u = a\cdot x + b\cdot y + c$\\
$v = d\cdot x + e\cdot y + f$\\
$u = a\cdot 1 + b\cdot 1 + c \;\; $ $\;\;
a+b+c = \frac{\sqrt{3}+1}{2}$ \\
$v = d\cdot 1 + e\cdot 1 + f\;\;$ $\;\;
d+e+f = \frac{\sqrt{3}-1}{2}$ \\
$u = a\cdot 0 + b\cdot 0 + c\;\;$ $\;\;
c = 1$\\
$v = d\cdot 0 + e\cdot 0 + f\;$ $\;\;
f = -1$\\
$u = a\cdot 1 + b\cdot 0 + c\;\;$ $\;\;
a+c = \frac{\sqrt{3}+2}{2}
$\\
$v = d\cdot 1 + e\cdot 0 + f\;\;$ $\;\;
d + f = \frac{-1}{2}
$\\
$a = \frac{\sqrt{3}+2}{2} - c = \frac{\sqrt{3}+2}{2} - 1 = \frac{\sqrt{3}}{2}$\\
$d = -\frac{1}{2} - f = -\frac{1}{2} - (-1) = \frac{1}{2}$\\
$b = \frac{\sqrt{3}+1}{2} - a - c = 
\frac{\sqrt{3}+1}{2} - \frac{\sqrt{3}}{2} - 1 =
-\frac{1}{2} 
$ \\
$e = \frac{\sqrt{3}-1}{2} -d -f =
\frac{\sqrt{3}-1}{2} -\frac{1}{2} -(-1) =
\frac{\sqrt{3}}{2}
$ \\\\
$a = \frac{\sqrt{3}}{2}$
$b = -\frac{1}{2} $ 
$c = 1$
$d = \frac{1}{2}$
$e = \frac{\sqrt{3}}{2}$ 
$f = -1$
$\begin{bmatrix}
\;\; \frac{\sqrt{3}}{2} \;\; & \;\;-\frac{1}{2}\;\; & \;\; 1 \;\;\\
\;\; \frac{1}{2} \;\; & \;\; \frac{\sqrt{3}}{2} \;\; & \;\; -1 \;\;\\
\;\; 0 \;\; & \;\; 0 \;\; & \;\; 1 \;\;\\
\end{bmatrix}$
\end{document}

